SP1Clean.lean
@@ -14,8 +14,8 @@ import SP1Clean.Reader.ITypeReader
 import SP1Clean.Reader.RTypeReader
 import SP1Clean.AddiChip.SailBridge
 import SP1Clean.AddChip.SailBridge
-import SP1Clean.SubChip
-import SP1Clean.SubwChip
+import SP1Clean.SubChip.SailBridge
+import SP1Clean.SubwChip.SailBridge
 import SP1Clean.AddwChip.SailBridge
 import SP1Clean.UTypeChip
 import SP1Clean.JalrChip
